Start working on elaboration details

ObcToClight/DataflowElab.v
@@ -10,21 +10,99 @@ Require Import Rustre.Ident.
 Module Export OpAux := OperatorsAux Interface.Op.
 Module Export Syn := SyntaxFun Ident.Ids Interface.Op.
 
+Require Import List.
+Import List.ListNotations.
+Open Scope list_scope.
+
+Require Import compcert.common.Errors.
+Local Open Scope error_monad_scope.
+
 (* Elaborate an AST into a well-typed Dataflow program. *)
 
+(* TODO: Should we just elaborate the constants in Lexer.mll ? *)
+
 (* CompCert: cparser/Elab: elab_int_constant + cfrontend/C2C: convertIkind *)
-Axiom elab_const_int : astloc -> string -> const.
+Parameter elab_const_int : astloc -> string -> constant.
 (* CompCert: cparser/Elab: elab_float_constant + cfrontend/C2C: convertIkind *)
-Axiom elab_const_float : floatInfo -> const.
+Parameter elab_const_float : floatInfo -> constant.
 (* CompCert: cparser/Elab: elab_char_constant + cfrontend/C2C: convertIkind *)
-Axiom elab_const_char : astloc -> bool -> list char_code -> const.
-                   
+Parameter elab_const_char : astloc -> bool -> list char_code -> constant.
+
+(* TODO: How to integrate with pos_of_str? *)
+(* TODO: Should we just turn identifiers into positives in Lexer.mll? *)
+Parameter ident_of_string : string -> ident.
+Parameter string_of_astloc : astloc -> String.string.
+
+Definition err_loc (loc: astloc) (m: errmsg) :=
+  MSG (string_of_astloc loc) :: MSG ": " :: m.  
+
 Module Type ELABORATION
        (Import Ids    : IDS)
        (Import Op     : OPERATORS)
+       (Import OpAux  : OPERATORS_AUX Op)
        (Import Syn    : SYNTAX Ids Op)
        (Import Typing : TYPING Ids Op Syn).
 
-  
+  Definition elab_constant (loc: astloc) (c: Ast.constant) : constant :=
+    match c with
+    | CONST_BOOL false  => Cint Integers.Int.zero Ctypes.IBool Ctypes.Signed
+    | CONST_BOOL true   => Cint Integers.Int.one Ctypes.IBool Ctypes.Signed
+    | CONST_INT s       => elab_const_int loc s
+    | CONST_FLOAT fi    => elab_const_float fi
+    | CONST_CHAR wide l => elab_const_char loc wide l
+    end.
+
+  Section ElabExpressions.
+
+    Variable env : PM.t type.
+
+    Definition has_type (x: ident) (ty: type) : bool :=
+      match PM.find x env with
+      | Some ty' => ty ==b ty'
+      | None => false
+      end.
+
+    Fixpoint elab_clock (loc: astloc) (ck: Ast.clock) : res clock :=
+      match ck with
+      | BASE => OK Cbase
+      | ON ck' b xs =>
+        let x := ident_of_string xs in
+        if has_type x bool_type then
+          do ck' <- elab_clock loc ck';
+             OK (Con ck' x b)
+        else Error (err_loc loc
+                       (CTX x :: msg " in clock is not declared as bool."))
+      end.
+
+  End ElabExpressions.
+
+  Lemma has_type_In:
+    forall env x ty,
+      has_type env x ty = true ->
+      In (x, ty) (PM.elements env).
+  Proof.
+    intros env x ty Hhty.
+    unfold has_type in Hhty.
+    destruct (PM.find x env) eqn:Hfind; try discriminate.
+    rewrite equiv_decb_equiv in Hhty.
+    rewrite <-Hhty in Hfind.
+    now apply PM.elements_correct in Hfind.
+  Qed.
+    
+  Lemma wt_elab_clock:
+    forall env loc ast_ck ck,
+      elab_clock env loc ast_ck = OK ck ->
+      wt_clock (PM.elements env) ck.
+  Proof.
+    induction ast_ck as [|ack IH]; simpl.
+    now injection 1; intro; subst; auto with dftyping.
+    destruct (has_type env (ident_of_string s) bool_type) eqn:Hstr.
+    2:discriminate 1.
+    intros ck Helab.
+    monadInv Helab.
+    constructor; auto.
+    apply has_type_In with (1:=Hstr).
+  Qed.
+    
 
 End ELABORATION.
